{-# OPTIONS --safe #-}
module Cubical.Data.Sum.Properties where

open import Cubical.Core.Everything
open import Cubical.Foundations.Prelude
open import Cubical.Foundations.HLevels
open import Cubical.Functions.Embedding
open import Cubical.Foundations.Equiv
open import Cubical.Foundations.Isomorphism
open import Cubical.Data.Empty
open import Cubical.Data.Nat
open import Cubical.Data.Sigma

open import Cubical.Data.Sum.Base

open Iso


private
  variable
    ℓa ℓb ℓc ℓd ℓe : Level
    A : Type ℓa
    B : Type ℓb
    C : Type ℓc
    D : Type ℓd
    E : A ⊎ B → Type ℓe


-- Path space of sum type
module ⊎Path {ℓ ℓ'} {A : Type ℓ} {B : Type ℓ'} where

  Cover : A ⊎ B → A ⊎ B → Type (ℓ-max ℓ ℓ')
  Cover (inl a) (inl a') = Lift {j = ℓ-max ℓ ℓ'} (a ≡ a')
  Cover (inl _) (inr _) = Lift ⊥
  Cover (inr _) (inl _) = Lift ⊥
  Cover (inr b) (inr b') = Lift {j = ℓ-max ℓ ℓ'} (b ≡ b')

  reflCode : (c : A ⊎ B) → Cover c c
  reflCode (inl a) = lift refl
  reflCode (inr b) = lift refl

  encode : ∀ c c' → c ≡ c' → Cover c c'
  encode c _ = J (λ c' _ → Cover c c') (reflCode c)

  encodeRefl : ∀ c → encode c c refl ≡ reflCode c
  encodeRefl c = JRefl (λ c' _ → Cover c c') (reflCode c)

  decode : ∀ c c' → Cover c c' → c ≡ c'
  decode (inl a) (inl a') (lift p) = cong inl p
  decode (inl a) (inr b') ()
  decode (inr b) (inl a') ()
  decode (inr b) (inr b') (lift q) = cong inr q

  decodeRefl : ∀ c → decode c c (reflCode c) ≡ refl
  decodeRefl (inl a) = refl
  decodeRefl (inr b) = refl

  decodeEncode : ∀ c c' → (p : c ≡ c') → decode c c' (encode c c' p) ≡ p
  decodeEncode c _ =
    J (λ c' p → decode c c' (encode c c' p) ≡ p)
      (cong (decode c c) (encodeRefl c) ∙ decodeRefl c)

  encodeDecode : ∀ c c' → (d : Cover c c') → encode c c' (decode c c' d) ≡ d
  encodeDecode (inl a) (inl _) (lift d) =
    J (λ a' p → encode (inl a) (inl a') (cong inl p) ≡ lift p) (encodeRefl (inl a)) d
  encodeDecode (inr a) (inr _) (lift d) =
    J (λ a' p → encode (inr a) (inr a') (cong inr p) ≡ lift p) (encodeRefl (inr a)) d

  Cover≃Path : ∀ c c' → Cover c c' ≃ (c ≡ c')
  Cover≃Path c c' =
    isoToEquiv (iso (decode c c') (encode c c') (decodeEncode c c') (encodeDecode c c'))

  isOfHLevelCover : (n : HLevel)
    → isOfHLevel (suc (suc n)) A
    → isOfHLevel (suc (suc n)) B
    → ∀ c c' → isOfHLevel (suc n) (Cover c c')
  isOfHLevelCover n p q (inl a) (inl a') = isOfHLevelLift (suc n) (p a a')
  isOfHLevelCover n p q (inl a) (inr b') =
    isOfHLevelLift (suc n) (isProp→isOfHLevelSuc n isProp⊥)
  isOfHLevelCover n p q (inr b) (inl a') =
    isOfHLevelLift (suc n) (isProp→isOfHLevelSuc n isProp⊥)
  isOfHLevelCover n p q (inr b) (inr b') = isOfHLevelLift (suc n) (q b b')

isEmbedding-inl : isEmbedding (inl {A = A} {B = B})
isEmbedding-inl w z = snd (compEquiv LiftEquiv (⊎Path.Cover≃Path (inl w) (inl z)))

isEmbedding-inr : isEmbedding (inr {A = A} {B = B})
isEmbedding-inr w z = snd (compEquiv LiftEquiv (⊎Path.Cover≃Path (inr w) (inr z)))

isOfHLevel⊎ : (n : HLevel)
  → isOfHLevel (suc (suc n)) A
  → isOfHLevel (suc (suc n)) B
  → isOfHLevel (suc (suc n)) (A ⊎ B)
isOfHLevel⊎ n lA lB c c' =
  isOfHLevelRetract (suc n)
    (⊎Path.encode c c')
    (⊎Path.decode c c')
    (⊎Path.decodeEncode c c')
    (⊎Path.isOfHLevelCover n lA lB c c')

isSet⊎ : isSet A → isSet B → isSet (A ⊎ B)
isSet⊎ = isOfHLevel⊎ 0

isGroupoid⊎ : isGroupoid A → isGroupoid B → isGroupoid (A ⊎ B)
isGroupoid⊎ = isOfHLevel⊎ 1

is2Groupoid⊎ : is2Groupoid A → is2Groupoid B → is2Groupoid (A ⊎ B)
is2Groupoid⊎ = isOfHLevel⊎ 2

⊎Iso : Iso A C → Iso B D → Iso (A ⊎ B) (C ⊎ D)
fun (⊎Iso iac ibd) (inl x) = inl (iac .fun x)
fun (⊎Iso iac ibd) (inr x) = inr (ibd .fun x)
inv (⊎Iso iac ibd) (inl x) = inl (iac .inv x)
inv (⊎Iso iac ibd) (inr x) = inr (ibd .inv x)
rightInv (⊎Iso iac ibd) (inl x) = cong inl (iac .rightInv x)
rightInv (⊎Iso iac ibd) (inr x) = cong inr (ibd .rightInv x)
leftInv (⊎Iso iac ibd) (inl x)  = cong inl (iac .leftInv x)
leftInv (⊎Iso iac ibd) (inr x)  = cong inr (ibd .leftInv x)

⊎-equiv : A ≃ C → B ≃ D → (A ⊎ B) ≃ (C ⊎ D)
⊎-equiv p q = isoToEquiv (⊎Iso (equivToIso p) (equivToIso q))

⊎-swap-Iso : Iso (A ⊎ B) (B ⊎ A)
fun ⊎-swap-Iso (inl x) = inr x
fun ⊎-swap-Iso (inr x) = inl x
inv ⊎-swap-Iso (inl x) = inr x
inv ⊎-swap-Iso (inr x) = inl x
rightInv ⊎-swap-Iso (inl _) = refl
rightInv ⊎-swap-Iso (inr _) = refl
leftInv ⊎-swap-Iso (inl _)  = refl
leftInv ⊎-swap-Iso (inr _)  = refl

⊎-swap-≃ : A ⊎ B ≃ B ⊎ A
⊎-swap-≃ = isoToEquiv ⊎-swap-Iso

⊎-assoc-Iso : Iso ((A ⊎ B) ⊎ C) (A ⊎ (B ⊎ C))
fun ⊎-assoc-Iso (inl (inl x)) = inl x
fun ⊎-assoc-Iso (inl (inr x)) = inr (inl x)
fun ⊎-assoc-Iso (inr x)       = inr (inr x)
inv ⊎-assoc-Iso (inl x)       = inl (inl x)
inv ⊎-assoc-Iso (inr (inl x)) = inl (inr x)
inv ⊎-assoc-Iso (inr (inr x)) = inr x
rightInv ⊎-assoc-Iso (inl _)       = refl
rightInv ⊎-assoc-Iso (inr (inl _)) = refl
rightInv ⊎-assoc-Iso (inr (inr _)) = refl
leftInv ⊎-assoc-Iso (inl (inl _))  = refl
leftInv ⊎-assoc-Iso (inl (inr _))  = refl
leftInv ⊎-assoc-Iso (inr _)        = refl

⊎-assoc-≃ : (A ⊎ B) ⊎ C ≃ A ⊎ (B ⊎ C)
⊎-assoc-≃ = isoToEquiv ⊎-assoc-Iso

⊎-⊥-Iso : Iso (A ⊎ ⊥) A
fun ⊎-⊥-Iso (inl x) = x
inv ⊎-⊥-Iso x       = inl x
rightInv ⊎-⊥-Iso _      = refl
leftInv ⊎-⊥-Iso (inl _) = refl

⊎-⊥-≃ : A ⊎ ⊥ ≃ A
⊎-⊥-≃ = isoToEquiv ⊎-⊥-Iso

Π⊎Iso : Iso ((x : A ⊎ B) → E x) (((a : A) → E (inl a)) × ((b : B) → E (inr b)))
fun Π⊎Iso f .fst a = f (inl a)
fun Π⊎Iso f .snd b = f (inr b)
inv Π⊎Iso (g1 , g2) (inl a) = g1 a
inv Π⊎Iso (g1 , g2) (inr b) = g2 b
rightInv Π⊎Iso (g1 , g2) i .fst a = g1 a
rightInv Π⊎Iso (g1 , g2) i .snd b = g2 b
leftInv Π⊎Iso f i (inl a) = f (inl a)
leftInv Π⊎Iso f i (inr b) = f (inr b)

Σ⊎Iso : Iso (Σ (A ⊎ B) E) ((Σ A (λ a → E (inl a))) ⊎ (Σ B (λ b → E (inr b))))
fun Σ⊎Iso (inl a , ea) = inl (a , ea)
fun Σ⊎Iso (inr b , eb) = inr (b , eb)
inv Σ⊎Iso (inl (a , ea)) = (inl a , ea)
inv Σ⊎Iso (inr (b , eb)) = (inr b , eb)
rightInv Σ⊎Iso (inl (a , ea)) = refl
rightInv Σ⊎Iso (inr (b , eb)) = refl
leftInv Σ⊎Iso (inl a , ea) = refl
leftInv Σ⊎Iso (inr b , eb) = refl

Π⊎≃ : ((x : A ⊎ B) → E x) ≃ ((a : A) → E (inl a)) × ((b : B) → E (inr b))
Π⊎≃ = isoToEquiv Π⊎Iso

Σ⊎≃ : (Σ (A ⊎ B) E) ≃ ((Σ A (λ a → E (inl a))) ⊎ (Σ B (λ b → E (inr b))))
Σ⊎≃ = isoToEquiv Σ⊎Iso

map-⊎ : (A → C) → (B → D) → A ⊎ B → C ⊎ D
map-⊎ f _ (inl a) = inl (f a)
map-⊎ _ g (inr b) = inr (g b)
