{-# OPTIONS --cubical --safe --guardedness #-}
module Cubical.Codata.Conat.Properties where

open import Cubical.Data.Unit
open import Cubical.Data.Sum
open import Cubical.Data.Empty

open import Cubical.Core.Everything
open import Cubical.Foundations.Equiv

open import Cubical.Codata.Conat.Base

Unwrap-prev : Conatâ€² -> Set
Unwrap-prev  zero   = Unit
Unwrap-prev (suc _) = Conat

unwrap-prev : (n : Conatâ€²) -> Unwrap-prev n
unwrap-prev  zero   = _
unwrap-prev (suc x) = x

private -- tests
  ğŸ˜ : Conat
  force ğŸ˜ = zero
  one  = succ ğŸ˜
  two  = succ one

  succOneâ‰¡two : succ one â‰¡ two
  succOneâ‰¡two i = two

  predTwoâ‰¡one : unwrap-prev (force two) â‰¡ one
  predTwoâ‰¡one i = one

âˆ : Conat
force âˆ = suc âˆ

âˆ+1â‰¡âˆ : succ âˆ â‰¡ âˆ
force (âˆ+1â‰¡âˆ _) = suc âˆ

âˆ+2â‰¡âˆ : succ (succ âˆ) â‰¡ âˆ
âˆ+2â‰¡âˆ = compPath (cong succ âˆ+1â‰¡âˆ) âˆ+1â‰¡âˆ

-- TODO: plus for conat, âˆ + âˆ â‰¡ âˆ

module Bisimulation where

  record _â‰ˆ_ (x y : Conat) : Set
  data _â‰ˆâ€²_ (x y : Conatâ€²) : Set
  _â‰ˆâ€²â€²_ : Conatâ€² â†’ Conatâ€² â†’ Set
  -- zero  â‰ˆâ€²â€² zero  = Unit
  suc x â‰ˆâ€²â€² suc y = x â‰ˆ y
  -- So impossible proofs are preserved
  x â‰ˆâ€²â€² y = x â‰¡ y

  record _â‰ˆ_ x y where
    coinductive
    field prove : force x â‰ˆâ€² force y

  data _â‰ˆâ€²_  x y where
    con : x â‰ˆâ€²â€² y â†’ x â‰ˆâ€² y

  open _â‰ˆ_ public

  bisim : âˆ€ {x y} â†’ x â‰ˆ y â†’ x â‰¡ y
  bisimâ€² : âˆ€ {x y} â†’ x â‰ˆâ€² y â†’ x â‰¡ y

  bisimâ€² {zero} {zero}  (con p) = p
  bisimâ€² {zero} {suc x} (con p) = p
  bisimâ€² {suc x} {zero} (con p) = p
  bisimâ€² {suc x} {suc y} (con eq) i = suc (bisim eq i)
  force (bisim eq i) = bisimâ€² (prove eq) i

  misib : âˆ€ {x y} â†’ x â‰¡ y â†’ x â‰ˆ y
  misibâ€² : âˆ€ {x y} â†’ x â‰¡ y â†’ x â‰ˆâ€² y

  misibâ€² {zero} {zero} p = con p
  misibâ€² {zero} {suc x} p = con p
  misibâ€² {suc x} {zero} p = con p
  -- misibâ€² {suc x} {suc y} p = con Î» where .prove â†’ misibâ€² (cong predâ€² p)
  misibâ€² {suc x} {suc y} p = con (misib (cong predâ€²â€² p))
  prove (misib xâ‰¡y) = misibâ€² (cong force xâ‰¡y)

  iso1 : âˆ€ {x y} â†’ (p : x â‰ˆ y) â†’ misib (bisim p) â‰¡ p
  iso1â€² : âˆ€ {x y} â†’ (p : x â‰ˆâ€² y) â†’ misibâ€² (bisimâ€² p) â‰¡ p

  iso1â€² {zero} {zero} (con p) i = con p
  iso1â€² {zero} {suc x} (con p) i = con p
  iso1â€² {suc x} {zero} (con p) i = con p
  iso1â€² {suc x} {suc y} p i = p
  prove (iso1 p i) = iso1â€² (prove p) i

  iso2 : âˆ€ {x y} â†’ (p : x â‰¡ y) â†’ bisim (misib p) â‰¡ p
  iso2â€² : âˆ€ {x y} â†’ (p : x â‰¡ y) â†’ bisimâ€² (misibâ€² p) â‰¡ p

  iso2â€² {zero} {zero} p _ = p
  iso2â€² {zero} {suc x} p _ = p
  iso2â€² {suc x} {zero} p _ = p
  iso2â€² {suc x} {suc y} p i j = suc (iso2 (cong predâ€²â€² p) i j)
  force (iso2 p i j) = iso2â€² (cong force p) i j

  pathâ‰ƒbisim : âˆ€ {x y} â†’ (x â‰¡ y) â‰ƒ (x â‰ˆ y)
  pathâ‰ƒbisim = isoToEquiv misib bisim iso2 iso1

  pathâ‰¡bisim : âˆ€ {x y} â†’ (x â‰¡ y) â‰¡ (x â‰ˆ y)
  pathâ‰¡bisim = ua pathâ‰ƒbisim
