{-# OPTIONS --cubical --no-import-sorts --safe #-}
module Cubical.HITs.Susp.Base where

open import Cubical.Foundations.Prelude
open import Cubical.Foundations.Equiv
open import Cubical.Foundations.Univalence
open import Cubical.Foundations.Isomorphism
open import Cubical.Foundations.Pointed

open import Cubical.Data.Bool
open import Cubical.Data.Empty

open import Cubical.HITs.S1 hiding (inv)
open import Cubical.HITs.S2
open import Cubical.HITs.S3

open Iso

data Susp {ℓ} (A : Type ℓ) : Type ℓ where
  north : Susp A
  south : Susp A
  merid : (a : A) → north ≡ south

∙Susp : ∀ {ℓ} (A : Type ℓ) → Pointed ℓ
∙Susp A = Susp A , north

BoolIsoSusp⊥ : Iso Bool (Susp ⊥)
fun BoolIsoSusp⊥ = λ {true  → north; false → south}
inv BoolIsoSusp⊥ = λ {north → true;  south → false}
rightInv BoolIsoSusp⊥ = λ {north → refl;  south → refl}
leftInv BoolIsoSusp⊥  = λ {true  → refl;  false → refl}

Bool≃Susp⊥ : Bool ≃ Susp ⊥
Bool≃Susp⊥ = isoToEquiv BoolIsoSusp⊥

SuspBool : Type₀
SuspBool = Susp Bool

SuspBool→S¹ : SuspBool → S¹
SuspBool→S¹ north = base
SuspBool→S¹ south = base
SuspBool→S¹ (merid false i) = loop i
SuspBool→S¹ (merid true i)  = base

S¹→SuspBool : S¹ → SuspBool
S¹→SuspBool base     = north
S¹→SuspBool (loop i) = (merid false ∙ sym (merid true)) i

SuspBool→S¹→SuspBool : (x : SuspBool) → Path _ (S¹→SuspBool (SuspBool→S¹ x)) x
SuspBool→S¹→SuspBool north = refl
SuspBool→S¹→SuspBool south = merid true
SuspBool→S¹→SuspBool (merid false i) j = hcomp (λ k → (λ { (j = i1) → merid false i
                                                         ; (i = i0) → north
                                                         ; (i = i1) → merid true (j ∨ ~ k)}))
                                               (merid false i)
SuspBool→S¹→SuspBool (merid true i) j = merid true (i ∧ j)

S¹→SuspBool→S¹ : (x : S¹) → SuspBool→S¹ (S¹→SuspBool x) ≡ x
S¹→SuspBool→S¹ base       = refl
S¹→SuspBool→S¹ (loop i) j = hfill (λ k → λ { (i = i0) → base
                                           ; (i = i1) → base })
                                  (inS (loop i)) (~ j)

S¹IsoSuspBool : Iso S¹ SuspBool
fun S¹IsoSuspBool      = S¹→SuspBool
inv S¹IsoSuspBool      = SuspBool→S¹
rightInv S¹IsoSuspBool = SuspBool→S¹→SuspBool
leftInv S¹IsoSuspBool  = S¹→SuspBool→S¹

S¹≃SuspBool : S¹ ≃ SuspBool
S¹≃SuspBool = isoToEquiv S¹IsoSuspBool

S¹≡SuspBool : S¹ ≡ SuspBool
S¹≡SuspBool = ua S¹≃SuspBool

-- Now the sphere

SuspS¹ : Type₀
SuspS¹ = Susp S¹

SuspS¹→S² : SuspS¹ → S²
SuspS¹→S² north = base
SuspS¹→S² south = base
SuspS¹→S² (merid base i) = base
SuspS¹→S² (merid (loop j) i) = surf i j

meridian-contraction : I → I → I → SuspS¹
meridian-contraction i j l = hfill (λ k → λ { (i = i0) → north
                                            ; (i = i1) → merid base (~ k)
                                            ; (j = i0) → merid base (~ k ∧ i)
                                            ; (j = i1) → merid base (~ k ∧ i) })
                                   (inS (merid (loop j) i)) l

S²→SuspS¹ : S² → SuspS¹
S²→SuspS¹ base = north
S²→SuspS¹ (surf i j) = meridian-contraction i j i1

S²→SuspS¹→S² : ∀ x → SuspS¹→S² (S²→SuspS¹ x) ≡ x
S²→SuspS¹→S² base k = base
S²→SuspS¹→S² (surf i j) k = SuspS¹→S² (meridian-contraction i j (~ k))

SuspS¹→S²→SuspS¹ : ∀ x → S²→SuspS¹ (SuspS¹→S² x) ≡ x
SuspS¹→S²→SuspS¹ north k = north
SuspS¹→S²→SuspS¹ south k = merid base k
SuspS¹→S²→SuspS¹ (merid base j) k = merid base (k ∧ j)
SuspS¹→S²→SuspS¹ (merid (loop j) i) k = meridian-contraction i j (~ k)

S²IsoSuspS¹ : Iso S² SuspS¹
fun S²IsoSuspS¹      = S²→SuspS¹
inv S²IsoSuspS¹      = SuspS¹→S²
rightInv S²IsoSuspS¹ = SuspS¹→S²→SuspS¹
leftInv S²IsoSuspS¹  = S²→SuspS¹→S²

S²≃SuspS¹ : S² ≃ SuspS¹
S²≃SuspS¹ = isoToEquiv S²IsoSuspS¹

S²≡SuspS¹ : S² ≡ SuspS¹
S²≡SuspS¹ = ua S²≃SuspS¹

-- And the 3-sphere

SuspS² : Type₀
SuspS² = Susp S²

SuspS²→S³ : SuspS² → S³
SuspS²→S³ north = base
SuspS²→S³ south = base
SuspS²→S³ (merid base i) = base
SuspS²→S³ (merid (surf j k) i) = surf i j k

meridian-contraction-2 : I → I → I → I → SuspS²
meridian-contraction-2 i j k l = hfill (λ m → λ { (i = i0) → north
                                                ; (i = i1) → merid base (~ m)
                                                ; (j = i0) → merid base (~ m ∧ i)
                                                ; (j = i1) → merid base (~ m ∧ i)
                                                ; (k = i0) → merid base (~ m ∧ i)
                                                ; (k = i1) → merid base (~ m ∧ i) })
                                       (inS (merid (surf j k) i)) l

S³→SuspS² : S³ → SuspS²
S³→SuspS² base = north
S³→SuspS² (surf i j k) = meridian-contraction-2 i j k i1

S³→SuspS²→S³ : ∀ x → SuspS²→S³ (S³→SuspS² x) ≡ x
S³→SuspS²→S³ base l = base
S³→SuspS²→S³ (surf i j k) l = SuspS²→S³ (meridian-contraction-2 i j k (~ l))

SuspS²→S³→SuspS² : ∀ x → S³→SuspS² (SuspS²→S³ x) ≡ x
SuspS²→S³→SuspS² north l = north
SuspS²→S³→SuspS² south l = merid base l
SuspS²→S³→SuspS² (merid base j) l = merid base (l ∧ j)
SuspS²→S³→SuspS² (merid (surf j k) i) l = meridian-contraction-2 i j k (~ l)

S³IsoSuspS² : Iso S³ SuspS²
fun S³IsoSuspS²      = S³→SuspS²
inv S³IsoSuspS²      = SuspS²→S³
rightInv S³IsoSuspS² = SuspS²→S³→SuspS²
leftInv S³IsoSuspS²  = S³→SuspS²→S³

S³≃SuspS² : S³ ≃ SuspS²
S³≃SuspS² = isoToEquiv S³IsoSuspS²

S³≡SuspS² : S³ ≡ SuspS²
S³≡SuspS² = ua S³≃SuspS²
