{-# OPTIONS --safe --experimental-lossy-unification #-}
module Cubical.ZCohomology.RingStructure.CupProduct where
open import Cubical.ZCohomology.Base
open import Cubical.ZCohomology.GroupStructure
open import Cubical.ZCohomology.Properties

open import Cubical.HITs.S1 hiding (_·_)
open import Cubical.HITs.Sn
open import Cubical.HITs.Susp
open import Cubical.HITs.SetTruncation renaming (rec2 to sRec2)
open import Cubical.HITs.Truncation renaming (rec to trRec)

open import Cubical.Foundations.HLevels
open import Cubical.Foundations.Prelude
open import Cubical.Foundations.Pointed
open import Cubical.Data.Int hiding (_+'_ ; +'≡+ ; _+_)
open import Cubical.Data.Nat

infixl 30 _·₀_
infixr 35 _⌣ₖ_
infixr 35 _⌣_

--- This definition of ℕ-addition removes some unnecessary transports.
_+'_ : ℕ → ℕ → ℕ
zero +' b = b
suc a +' zero = suc a
suc a +' suc b = 2 + (a + b)

+'≡+ : (n m : ℕ) → n +' m ≡ n + m
+'≡+ zero m = refl
+'≡+ (suc n) zero = cong suc (sym (+-comm n zero))
+'≡+ (suc n) (suc m) = cong suc (sym (+-suc n m))

-- Cup product with one integer (K₀) argument
_·₀_ : {n : ℕ} (m : ℤ) → coHomK n → coHomK n
_·₀_ {n = n} (pos zero) x = 0ₖ _
_·₀_ {n = n} (pos (suc m)) x = x +ₖ (pos m ·₀ x)
_·₀_ {n = n} (negsuc zero) x = -ₖ x
_·₀_ {n = n} (negsuc (suc m)) x = (negsuc m ·₀ x) -ₖ x

·₀-0ₖ : {n : ℕ} (m : ℤ) → _·₀_ m (0ₖ n) ≡ 0ₖ n
·₀-0ₖ (pos zero) = refl
·₀-0ₖ (pos (suc n)) = cong (0ₖ _ +ₖ_) (·₀-0ₖ (pos n)) ∙ rUnitₖ _ (0ₖ _)
·₀-0ₖ (negsuc zero) = -0ₖ
·₀-0ₖ (negsuc (suc n)) = cong (λ x → x -ₖ (0ₖ _)) (·₀-0ₖ (negsuc n)) ∙ rCancelₖ _ (0ₖ _)

-- Pointed version first (enables truncation elimination)
⌣ₖ∙ : (n m : ℕ) → coHomK n → coHomK-ptd m →∙ coHomK-ptd (n +' m)
fst (⌣ₖ∙ zero m a) b = a ·₀ b
snd (⌣ₖ∙ zero m a) = ·₀-0ₖ a
fst (⌣ₖ∙ (suc n) zero a) b = b ·₀ a
snd (⌣ₖ∙ (suc n) zero a) = refl
⌣ₖ∙ (suc n) (suc m) = trRec (isOfHLevel↑∙ (suc n) m) (cup n m)
  where
  cup : (n m : ℕ) → S₊ (suc n) → coHomK-ptd (suc m) →∙ coHomK-ptd (suc (suc (n + m)))
  fst (cup zero m base) _ = 0ₖ _
  fst (cup zero m (loop i)) x = Kn→ΩKn+1 _ x i
  fst (cup (suc n) m north) _ = 0ₖ _
  fst (cup (suc n) m south) _ = 0ₖ _
  fst (cup (suc n) m (merid a i)) x = Kn→ΩKn+1 _ (fst (cup n m a) x) i
  snd (cup zero m base) = refl
  snd (cup zero m (loop i)) k = Kn→ΩKn+10ₖ _ k i
  snd (cup (suc n) m north) = refl
  snd (cup (suc n) m south) = refl
  snd (cup (suc n) m (merid a i)) k = (cong (Kn→ΩKn+1 _) (snd (cup n m a)) ∙ Kn→ΩKn+10ₖ _) k i

-- Non pointed version
_⌣ₖ_ : {n m : ℕ} → coHomK n → coHomK m → coHomK (n +' m)
_⌣ₖ_ {n = n} {m = m} x y = fst (⌣ₖ∙ n m x) y

-- Doubly pointed version
⌣ₖ∙∙ : (n m : ℕ) → coHomK-ptd n →∙ (coHomK-ptd m →∙ coHomK-ptd (n +' m) ∙)
fst (⌣ₖ∙∙ n m) = ⌣ₖ∙ n m
fst (snd (⌣ₖ∙∙ zero zero) i) x = 0
fst (snd (⌣ₖ∙∙ zero (suc m)) i) x = 0ₖ _
fst (snd (⌣ₖ∙∙ (suc n) zero) i) x = ·₀-0ₖ x i
fst (snd (⌣ₖ∙∙ (suc zero) (suc m)) i) x = 0ₖ _
fst (snd (⌣ₖ∙∙ (suc (suc n)) (suc m)) i) x = 0ₖ _
snd (snd (⌣ₖ∙∙ zero zero) i) = refl
snd (snd (⌣ₖ∙∙ zero (suc m)) i) = refl
snd (snd (⌣ₖ∙∙ (suc n) zero) i) = refl
snd (snd (⌣ₖ∙∙ (suc zero) (suc m)) i) = refl
snd (snd (⌣ₖ∙∙ (suc (suc n)) (suc m)) i) = refl

-- Cup product
_⌣_ : ∀ {ℓ} {A : Type ℓ} {n m : ℕ} → coHom n A → coHom m A → coHom (n +' m) A
_⌣_ = sRec2 squash₂ λ f g → ∣ (λ x → f x ⌣ₖ g x) ∣₂
