module Cubical.Algebra.CommRing.Instances.Fast.Int where

open import Cubical.Foundations.Prelude

open import Cubical.Algebra.CommRing
open import Cubical.Algebra.Ring.Properties
open import Cubical.Data.Fast.Int as Int renaming (_+_ to _+â„¤_; _Â·_ to _Â·â„¤_ ; -_ to -â„¤_)

open import Cubical.Data.Nat hiding (_+_; _Â·_)
import Cubical.Data.Nat as â„•

open CommRingStr using (0r ; 1r ; _+_ ; _Â·_ ; -_ ; isCommRing)

â„¤CommRing : CommRing â„“-zero
fst â„¤CommRing = â„¤
0r (snd â„¤CommRing) = pos 0
1r (snd â„¤CommRing) = pos 1
_+_ (snd â„¤CommRing) = _+â„¤_
_Â·_ (snd â„¤CommRing) = _Â·â„¤_
- snd â„¤CommRing = -â„¤_
isCommRing (snd â„¤CommRing) = isCommRingâ„¤
  where
  abstract
    isCommRingâ„¤ : IsCommRing (pos 0) (pos 1) _+â„¤_ _Â·â„¤_ -â„¤_
    isCommRingâ„¤ = makeIsCommRing isSetâ„¤ Int.+Assoc +IdR
                                 -Cancel Int.+Comm Int.Â·Assoc
                                 Int.Â·IdR Â·DistR+ Int.Â·Comm


private
 variable
  â„“ : Level

module CanonicalHomFromâ„¤ (ring : CommRing â„“) where

 module R where
  open CommRingStr (snd ring) public
  open RingTheory (CommRingâ†’Ring ring) public

 module ğ™ = CommRingStr (snd â„¤CommRing)

 suc-fromâ„• : âˆ€ x â†’ R.fromâ„• (suc x) â‰¡ R.1r R.+ R.fromâ„• x
 suc-fromâ„• zero = sym (R.+IdR R.1r)
 suc-fromâ„• (suc x) = refl


 fromâ„•-pres-+ : (x y : â„•) â†’ R.fromâ„• (x â„•.+ y) â‰¡ R.fromâ„• x R.+ R.fromâ„• y
 fromâ„•-pres-+ zero y = sym (R.+IdL _)
 fromâ„•-pres-+ (suc zero) y = suc-fromâ„• y
 fromâ„•-pres-+ (suc (suc x)) y =  cong (R.1r R.+_) (fromâ„•-pres-+ (suc x) y) âˆ™ R.+Assoc _ _ _

 
 fromâ„¤-pres-minus : (x : â„¤) â†’ R.fromâ„¤ (-â„¤ x) â‰¡ R.- R.fromâ„¤ x
 fromâ„¤-pres-minus (pos zero) = sym R.0Selfinverse
 fromâ„¤-pres-minus (pos (suc n)) = refl
 fromâ„¤-pres-minus (negsuc n) = sym (R.-Idempotent _)


 suc-fromâ„¤ : âˆ€ z â†’ R.fromâ„¤ (1 +â„¤ z) â‰¡ R.1r R.+ R.fromâ„¤ (z)
 suc-fromâ„¤ (pos n) = suc-fromâ„• n
 suc-fromâ„¤ (negsuc zero) = sym (R.+InvR R.1r)
   
 suc-fromâ„¤ (negsuc (suc n)) =
      sym (R.+IdL' _ _ (R.+InvR _))
   âˆ™âˆ™ sym (R.+Assoc _ _ _)
   âˆ™âˆ™ cong (R.1r R.+_) (R.-Dist _ _)
   
 fromâ„¤-pres-+' : (n nâ‚ : â„•) â†’
      R.fromâ„¤ (pos n +â„¤ negsuc nâ‚) â‰¡
      R.fromâ„¤ (pos n) R.+ R.fromâ„¤ (negsuc nâ‚)
 fromâ„¤-pres-+' zero nâ‚ = sym (R.+IdL _)
 fromâ„¤-pres-+' (suc n) nâ‚ =  
    (cong R.fromâ„¤ (sym (ğ™.+Assoc 1 (pos n) (negsuc nâ‚)))
     âˆ™ suc-fromâ„¤ (pos n +â„¤ negsuc nâ‚))
    âˆ™âˆ™ cong (R.1r R.+_) (fromâ„¤-pres-+' n nâ‚)
    âˆ™âˆ™ R.+Assoc _ _ _
    âˆ™ cong (R._+ R.fromâ„¤ (negsuc nâ‚))
     (sym (suc-fromâ„• n))
 
 fromâ„¤-pres-+ : (x y : â„¤) â†’ R.fromâ„¤ (x +â„¤ y) â‰¡ R.fromâ„¤ x R.+ R.fromâ„¤ y
 fromâ„¤-pres-+ (pos n) (pos nâ‚) = fromâ„•-pres-+ n nâ‚
 fromâ„¤-pres-+ (pos n) (negsuc nâ‚) = fromâ„¤-pres-+' n nâ‚
 fromâ„¤-pres-+ (negsuc n) (pos nâ‚) = 
       fromâ„¤-pres-+' nâ‚ n
     âˆ™ R.+Comm _ _
    
 fromâ„¤-pres-+ (negsuc n) (negsuc nâ‚) = 
    cong (R.-_)
       (cong (R.1r R.+_) (cong R.fromâ„• (sym (â„•.+-suc n nâ‚)))
        âˆ™ sym (suc-fromâ„• (n â„•.+ suc nâ‚))
          âˆ™ fromâ„•-pres-+ (suc n) (suc nâ‚))
   âˆ™ sym (R.-Dist _ _)


 fromâ„•-pres-Â· : (x y : â„•) â†’ R.fromâ„• (x â„•.Â· y) â‰¡ R.fromâ„• x R.Â· R.fromâ„• y
 fromâ„•-pres-Â· zero y = sym (R.0LeftAnnihilates _)
 fromâ„•-pres-Â· (suc x) y = 
    fromâ„•-pres-+ y (x â„•.Â· y)
   âˆ™âˆ™ congâ‚‚ (R._+_) (sym (R.Â·IdL _)) (fromâ„•-pres-Â· x y) 
   âˆ™âˆ™ sym (R.Â·DistL+ _ _ _)
   âˆ™ cong (R._Â· R.fromâ„• y) (sym (suc-fromâ„• x))

 fromâ„¤-pres-Â· : (x y : â„¤) â†’ R.fromâ„¤ (x Â·â„¤ y) â‰¡ R.fromâ„¤ x R.Â· R.fromâ„¤ y
 fromâ„¤-pres-Â· (pos n) (pos nâ‚) = fromâ„•-pres-Â· n nâ‚
 fromâ„¤-pres-Â· (pos n) (negsuc nâ‚) =
        cong R.fromâ„¤ (sym (-DistRÂ· (pos n) (pos (suc nâ‚))))
     âˆ™âˆ™ (fromâ„¤-pres-minus (pos (n â„•.Â· suc nâ‚))
        âˆ™ cong R.-_ (fromâ„•-pres-Â· n (suc nâ‚)))
     âˆ™âˆ™ sym (R.-DistRÂ· _ _)

 fromâ„¤-pres-Â· (negsuc n) (pos nâ‚) =
           cong R.fromâ„¤ (sym (-DistLÂ· (pos (suc n)) (pos nâ‚)))
     âˆ™âˆ™ (fromâ„¤-pres-minus (pos ((suc n) â„•.Â· nâ‚))
        âˆ™ cong R.-_ (fromâ„•-pres-Â· (suc n) nâ‚))
     âˆ™âˆ™ sym (R.-DistLÂ· _ _)

 fromâ„¤-pres-Â· (negsuc n) (negsuc nâ‚) =
        fromâ„•-pres-Â· (suc n) (suc nâ‚)
    âˆ™âˆ™ congâ‚‚ R._Â·_ (sym (R.-Idempotent _)) refl
    âˆ™âˆ™ R.-SwapÂ· _ _
 
 isHomFromâ„¤ : IsCommRingHom (â„¤CommRing .snd) R.fromâ„¤ (ring .snd)
 isHomFromâ„¤ .IsCommRingHom.pres0 = refl
 isHomFromâ„¤ .IsCommRingHom.pres1 = refl
 isHomFromâ„¤ .IsCommRingHom.pres+ = fromâ„¤-pres-+
 isHomFromâ„¤ .IsCommRingHom.presÂ· = fromâ„¤-pres-Â·
 isHomFromâ„¤ .IsCommRingHom.pres- = fromâ„¤-pres-minus
